src/Experiments/SpecificCurve25519.v
@@ -1,17 +1,133 @@
-Require Import Crypto.Util.Notations Coq.ZArith.BinInt.
+Require Import Coq.Classes.RelationClasses.
+Require Import Crypto.Util.Notations Crypto.Util.Tactics Coq.ZArith.BinInt.
 Require Import Crypto.Spec.ModularArithmetic.
+Require Import Crypto.ModularArithmetic.PrimeFieldTheorems.
 Require Import Crypto.Specific.GF25519.
 Require Import Crypto.Experiments.SpecEd25519.
 Require Import Crypto.CompleteEdwardsCurve.ExtendedCoordinates.
-Local Infix "<<" := Z.shiftr.
+Require Import Crypto.CompleteEdwardsCurve.CompleteEdwardsCurveTheorems.
+Require Import Crypto.Util.Decidable.
+
+Require Import Crypto.Experiments.EdDSARefinement.
+Require Import Crypto.Spec.ModularWordEncoding.
+Require Import Crypto.Encoding.PointEncodingPre.
+
+Require Import BinNat.
+Require Import Crypto.Util.IterAssocOp.
+
+Require Import Bedrock.Word.
+
+Local Infix ">>" := Z.shiftr.
 Local Infix "&" := Z.land.
 
 Section Curve25519.
+  Axiom fe25519_sign_bit : fe25519 -> bool.
+  Axiom convert_fe25519_to_wire : Encoding.CanonicalEncoding fe25519 (Word.word 255).
 
   Definition twice_d : fe25519 := Eval vm_compute in
     @ModularBaseSystem.encode modulus params25519 (d + d)%F.
+  Definition a : fe25519 := Eval vm_compute in
+    @ModularBaseSystem.encode modulus params25519 a.
+  Definition d : fe25519 := Eval vm_compute in
+    @ModularBaseSystem.encode modulus params25519 d.
 
-  Definition ge25519_add :=
-    Eval cbv beta delta [Extended.add_coordinates fe25519 add mul sub ModularBaseSystemOpt.Let_In] in
-      @Extended.add_coordinates fe25519 add sub mul twice_d.
+  Lemma prm25519 :
+    @E.twisted_edwards_params fe25519
+                              ModularBaseSystem.eq ModularBaseSystem.zero ModularBaseSystem.one add mul
+                              a d.
+  Proof.
+  Admitted.
+
+  Lemma Hphi : @Algebra.Ring.is_homomorphism
+                 (F q) (@eq (F q)) 1%F (@F.add q) (@F.mul q) fe25519
+                 (@ModularBaseSystem.eq modulus params25519) (@ModularBaseSystem.one modulus params25519) add mul
+                 (@ModularBaseSystem.encode modulus params25519).
+  Admitted.
+
+  Lemma phi_nonzero : forall x : F q,
+      x <> 0%F -> ~ ModularBaseSystem.eq (@ModularBaseSystem.encode _ params25519 x) ModularBaseSystem.zero.
+  Admitted.
+
+  Definition ge25519 :=
+    @Extended.point
+      fe25519 (@ModularBaseSystem.eq modulus params25519)
+      (@ModularBaseSystem.zero modulus params25519) (@ModularBaseSystem.one modulus params25519) add mul
+      (@ModularBaseSystem.div modulus params25519) a d.
+
+  Lemma HKa : ModularBaseSystem.eq a (ModularBaseSystem.opp ModularBaseSystem.one). vm_decide_no_check. Qed.
+  Lemma Hd : ModularBaseSystem.eq (ModularBaseSystem.encode SpecEd25519.d) d. vm_decide_no_check. Qed.
+
+  Definition ge25519_from_ref : E.point -> _ := fun P => Extended.ref_phi(phi:=ModularBaseSystem.encode)(fieldF:=F.field_modulo q)(fieldK:=field25519)(Kd:=d)(Ka:=a)(Hd:=Hd)(HKa:=HKa)(HFa:=eq_refl)(Hphi:=Hphi)(phi_nonzero:=phi_nonzero) (Extended.from_twisted P).
+
+  Definition ge25519_mul_N : N -> ge25519 -> ge25519  :=
+    iter_op
+      (op:=Extended.add(field:=field25519)(prm:=prm25519)(a_eq_minus1:=eq_refl)(Htwice_d:=eq_refl))
+      (id:=Extended.zero(field:=field25519)(prm:=prm25519))
+      N.testbit_nat
+      (Z.to_nat (Z.log2_up l))
+  .
+
+  Definition twisted25519_to_wire P : Word.word 256 :=
+    point_enc(F:=fe25519)(eq:=ModularBaseSystem.eq)(one:=ModularBaseSystem.one)
+             (add:=GF25519.add)(mul:=GF25519.mul)(a:=a)(d:=d)(sz:=255)(sign_bit:=fe25519_sign_bit) convert_fe25519_to_wire P.
+
+  Definition ge25519_to_wire := fun P => twisted25519_to_wire (Extended.to_twisted(field:=field25519) P).
+  Lemma ge25519_to_wire_correct : forall P : E.point, Eenc P = ge25519_to_wire (ge25519_from_ref P).
+  Admitted.
+  Definition ge25519_coords_B := Eval vm_compute in proj1_sig (ge25519_from_ref B).
+  Axiom admit : forall {T}, T.
+  Definition ge25519_B : ge25519 := exist _ ge25519_coords_B admit.
+  Definition ge25519_coords_zero := Eval vm_compute in proj1_sig (ge25519_from_ref E.zero).
+  Definition ge25519_zero : ge25519 := exist _ ge25519_coords_zero admit.
+  
+  (*
+  Time
+  Definition ge25519_coords_lB := Eval native_compute in
+        proj1_sig (ge25519_mul_N (Z.to_N l_Z) ge25519_B).
+  (* Finished transaction in 1091.517 secs (1091.353u,0.196s) (successful) *)
+
+  Definition twisted25519_coords_lB := Eval native_compute in proj1_sig (Extended.to_twisted(field:=field25519)(prm:=prm25519) (exist _ (ge25519_coords_lB) admit)).
+  *)
+
+  Definition SRepDecModL (h:word (b + b)): N :=
+    N.modulo (wordToN h) (Z.to_N l).
+
+  Import NPeano Nat.
+  Local Infix "mod" := modulo (at level 40, no associativity).
+  Lemma N_of_nat_mod a b : N.of_nat (a mod b) = N.modulo (N.of_nat a) (N.of_nat b).
+  Admitted.
+  
+  Definition ge25519_add := @Extended.add _ _ _ _ _ _ _ _ _ _ _ _
+                                          field25519 prm25519 admit admit admit.
+
+  Definition ge25519_opp := Extended.opp(field:=field25519)(prm:=prm25519).
+
+  (*
+  Goal
+    forall
+      Edec
+      SRepDec 
+      ERepEnc
+      ERepDec 
+      ERepGroup ERepHomomorphism
+      ERepEnc_correct ERepDec_correct SRepDecModL_correct SRepERepMul_correct
+      Proper_SRepERepMul SRepDec_correct Proper_ERepEnc
+      
+      ,
+      forall x, x =
+    @verify_using_representation
+(@E.point (F q) Logic.eq 1%F F.add F.mul (F.opp 1) SpecEd25519.d)
+E.eq E.add E.zero E.opp E.mul b H c n l B _ _
+Ed25519
+Edec (@Encoding.dec _ _ FlEncoding)
+ge25519 Extended.eq ge25519_add ge25519_zero ge25519_opp ERepGroup ge25519_from_ref ERepHomomorphism
+ERepEnc ERepEnc_correct Proper_ERepEnc ERepDec ERepDec_correct
+
+N Logic.eq
+_ F.to_N SRepDecModL SRepDecModL_correct ge25519_mul_N
+SRepERepMul_correct Proper_SRepERepMul SRepDec SRepDec_correct
+-> True.
+    intros; exact I.
+  Qed.
+   *)
 End Curve25519.
